Fix the clrewrite tactic, change Relations.v to work on relations in Prop only, and get rid of the "relation" definition which makes unification fail blatantly. Replace it with a notation :) In its current state, the new tactic seems ready for larger tests.
git-svn-id: svn+ssh://scm.gforge.inria.fr/svn/coq/trunk@10543 85f007b7-540e-0410-9357-904b9bb8a0f7

tactics/eauto.mli
@@ -61,6 +61,9 @@ end
 val full_eauto_gls : bool -> bool * int -> constr list -> goal list sigma * validation -> 
   goal list sigma * validation
 
+val resolve_all_evars_once : bool -> bool * int -> env -> (evar -> evar_info -> bool) -> evar_defs ->
+  evar_defs
+
 val resolve_all_evars : bool -> bool * int -> env -> (evar -> evar_info -> bool) -> evar_defs ->
   evar_defs
 
